src/coq/Handlers/Serialization.v
@@ -46,6 +46,23 @@ Module Type ITOP(Addr:MemoryAddress.ADDRESS)(PROV:PROVENANCE(Addr)).
   Parameter int_to_ptr : Z -> PROV.Prov -> Addr.addr.
 End ITOP.
 
+
+Require Import Vellvm.Utils.IntMaps.
+Inductive uvalue (addr : Type) (memory : Type) :=
+| UVALUE_Addr (a : addr)
+| UVALUE_Load (t : dtyp) (a : uvalue addr memory) (m : memory).
+
+Definition store_id := nat.
+
+Inductive SByte (addr : Type) (memory : Type) :=
+| UByte (uv : uvalue addr memory) (idx : uvalue addr memory) (sid : store_id).
+
+Require Import ZArith.
+
+
+Inductive memory (addr : Type) :=
+| Memory (m : IntMap (SByte addr (memory addr))).
+
 Module Make(Addr:MemoryAddress.ADDRESS)(LLVMIO: LLVM_INTERACTIONS(Addr))(SIZEOF: Sizeof)(PTOI:PTOI(Addr))(PROVENANCE:PROVENANCE(Addr))(ITOP:ITOP(Addr)(PROVENANCE)).
 
   Import LLVMIO.
@@ -56,14 +73,23 @@ Module Make(Addr:MemoryAddress.ADDRESS)(LLVMIO: LLVM_INTERACTIONS(Addr))(SIZEOF:
   Import DV.
   Open Scope list.
 
+  Variable ptr_size : nat.
+  Variable datalayout : DataLayout.
+
+  Variable mem_type : Type.
+  Variable eq_mem_type : mem_type -> mem_type -> Prop.
+  Variable eqb_mem_type : mem_type -> mem_type -> bool.
+  Instance mem_type_reldec : RelDec.RelDec eq_mem_type
+    := @RelDec.Build_RelDec mem_type eq_mem_type eqb_mem_type.
+
+
   Definition addr := Addr.addr.
+  Definition uvalue := @uvalue mem_type.
 
   (* TODO: move this? *)
   Inductive SByte :=
   | UByte (uv : uvalue) (dt : dtyp) (idx : uvalue) (sid : store_id) : SByte.
-
-  Variable ptr_size : nat.
-  Variable datalayout : DataLayout.
+  
 
   Definition endianess : Endianess
     := dl_endianess datalayout.
@@ -418,7 +444,8 @@ Module Make(Addr:MemoryAddress.ADDRESS)(LLVMIO: LLVM_INTERACTIONS(Addr))(SIZEOF:
        | UVALUE_ShuffleVector _ _ _
        | UVALUE_ExtractValue _ _
        | UVALUE_InsertValue _ _ _
-       | UVALUE_Select _ _ _ =>
+       | UVALUE_Select _ _ _
+       | UVALUE_Load _ _ _ =>
          sid <- fresh_sid;;
          ret (to_ubytes uv dt sid)
 
@@ -1125,7 +1152,7 @@ Ltac uvalue_eq_dec_refl_true :=
   rewrite rel_dec_eq_true; [|exact eq_dec_uvalue_correct|reflexivity].
 
 Ltac solve_guards_all_bytes :=
-  try rewrite N.eqb_refl; try rewrite Z.eqb_refl; uvalue_eq_dec_refl_true; cbn.
+  try rewrite N.eqb_refl; try rewrite Z.eqb_refl; try uvalue_eq_dec_refl_true; cbn.
 
 Lemma all_bytes_helper_app :
   forall  sbytes sbytes2 start sid uv,
@@ -1167,6 +1194,19 @@ Proof.
       rewrite map_length.
       rewrite Nseq_length.
       solve_guards_all_bytes.
+
+      rewrite rel_dec_eq_true.
+      * cbn. reflexivity.
+      * Set Printing Implicit.
+
+        
+
+
+Ltac uvalue_eq_dec_refl_true :=
+  rewrite rel_dec_eq_true; [|exact eq_dec_uvalue_correct|reflexivity].
+
+      [|exact eq_dec_uvalue_correct|reflexivity].
+      solve_guards_all_bytes
       reflexivity.
 Qed.
 
